1. added lexicographic induction version for LambdaANF and 2. fixed name

theories/LambdaANF/CompLex.v
@@ -7,15 +7,15 @@ Require Import Lia.
 From Hammer Require Import Hammer Tactics Reflect.
 
 From Common Require Import Util RelComp.
-From LambdaANF Require Import ANF Refl.
+From LambdaANF Require Import ANF ANFLex Util Tactics ReflLex.
 
-(* Compositionality of The Reflexive Pipeline Based on [Refl0.related_top] *)
+(* Compositionality of The Reflexive Pipeline Based on [related_top] *)
 
 (* Adequacy / Preservation of Termination *)
 (* Behavioral Refinement *)
 (* Linking Preservation *)
 
-Section Refl0Comp.
+Section Comp.
 
   Definition Top_n := Comp related_top.
 
@@ -28,7 +28,8 @@ Section Refl0Comp.
   Lemma V_n_refl n v :
     V_n n v v.
   Proof.
-    induction n; intros.
+    revert v.
+    induction n; prog.
     - constructor.
     - econstructor.
       + intros. eapply refl_V; eauto.
@@ -64,6 +65,7 @@ Section Refl0Comp.
       apply V_n_refl; auto.
     - pose proof (H 0) as Hr.
       destruct c2; simpl in Hr; try contradiction.
+      rewrite V_eq in Hr.
       edestruct IHComp as [v2 [Heq1 HVn]]; subst; eauto.
       eexists; split; eauto.
       econstructor.
@@ -99,12 +101,22 @@ Section Refl0Comp.
       eapply Included_trans; eauto.
   Qed.
 
-  Lemma G_n_subset n Γ1 Γ2 ρ1 ρ2 :
-    G_n n Γ1 ρ1 ρ2 ->
+  Lemma G_top_subset i Γ1 ρ1 Γ2 ρ2 :
+    G_top i Γ1 ρ1 ρ2 ->
     Γ2 \subset Γ1 ->
-    G_n n Γ2 ρ1 ρ2.
+    G_top i Γ2 ρ1 ρ2.
+  Proof.
+    unfold G_top.
+    intros; eauto.
+  Qed.
+
+  Lemma G_n_subset n Γ1 Γ2 ρ2 ρ3 :
+    G_n n Γ1 ρ2 ρ3 ->
+    Γ2 \subset Γ1 ->
+    G_n n Γ2 ρ2 ρ3.
   Proof.
     intros H.
+    revert Γ2.
     induction H; simpl; intros.
     - constructor.
     - econstructor.
@@ -113,7 +125,7 @@ Section Refl0Comp.
       + eapply IHComp; eauto.
   Qed.
 
-End Refl0Comp.
+End Comp.
 
 Section Adequacy.
 
@@ -167,6 +179,7 @@ Section Adequacy.
   Proof.
     intros.
     edestruct Top_n_adequacy with (ρ1 := ρ1) as [j2 [r2 [Hr2 HR]]]; eauto.
+    inv H1.
     edestruct R_n_Res_inv as [v2 [Heq HVn]]; eauto; subst.
     eexists; eexists; split; eauto.
   Qed.
@@ -175,22 +188,52 @@ End Adequacy.
 
 Section Refinement.
 
-  Inductive val_ref : val -> val -> Prop :=
-  | Ref_Vfun :
-    forall f1 ρ1 xs1 e1 f2 ρ2 xs2 e2,
-      val_ref (Vfun f1 ρ1 xs1 e1) (Vfun f2 ρ2 xs2 e2)
+  Fixpoint val_ref' (v1 v2 : val) : Prop:=
+    let fix Forall2_aux vs1 vs2 :=
+        match vs1, vs2 with
+        | [], [] => True
+        | v1 :: vs1, v2 :: vs2 =>
+          val_ref' v1 v2 /\ Forall2_aux vs1 vs2
+        | _, _ => False
+        end
+    in
+    match v1, v2 with
+    | Vconstr c1 vs1, Vconstr c2 vs2 =>
+        c1 = c2 /\ Forall2_aux vs1 vs2
+    | Vfun _ _ _ _, Vfun _ _ _ _ => True
+    | _, _ => False
+    end.
 
-  | Ref_Vconstr_nil :
-    forall c,
-      val_ref (Vconstr c []) (Vconstr c [])
+  Definition val_ref (v1 v2 : val) : Prop:=
+    match v1, v2 with
+    | Vconstr c1 vs1, Vconstr c2 vs2 =>
+        c1 = c2 /\ Forall2 val_ref' vs1 vs2
+    | Vfun _ _ _ _, Vfun _ _ _ _ => True
+    | _, _ => False
+    end.
 
-  | Ref_Vconstr_cons :
-    forall c v1 v2 vs1 vs2,
-      val_ref v1 v2 ->
-      val_ref (Vconstr c vs1) (Vconstr c vs2) ->
-      val_ref (Vconstr c (v1 :: vs1)) (Vconstr c (v2 :: vs2)).
+  Lemma val_ref_eq v1 v2 :
+    val_ref' v1 v2 <-> val_ref v1 v2.
+  Proof.
+    destruct v1; destruct v2; simpl; try easy;
+    split; intros H1; split; eauto.
+    + destruct H1; auto.
+    + destruct H1 as [Hc HF]; subst.
+      revert l0 HF. induction l; intros l0 H2; destruct l0; intros; eauto; inv H2.
+      constructor. easy. eauto.
+    + destruct H1; auto.
+    + destruct H1 as [Hc HF]; subst.
+      induction HF; auto.
+  Qed.
 
-  Hint Constructors val_ref : core.
+  Lemma val_ref_eq_Forall vs1 vs2 :
+    Forall2 val_ref' vs1 vs2 <-> Forall2 val_ref vs1 vs2.
+  Proof.
+    split; intros H; induction H; simpl; auto;
+      constructor; auto.
+    - rewrite <- val_ref_eq; auto.
+    - rewrite val_ref_eq; auto.
+  Qed.
 
   Lemma val_ref_Vconstr c vs1 vs2 :
     Forall2 val_ref vs1 vs2 ->
@@ -198,70 +241,51 @@ Section Refinement.
   Proof.
     intros.
     induction H; simpl; auto.
+    repeat (split; auto).
+    constructor.
+    rewrite val_ref_eq; auto.
+    rewrite val_ref_eq_Forall; auto.
   Qed.
 
   Lemma val_ref_refl v :
     val_ref v v.
   Proof.
-    induction v using val_ind'; auto.
+    induction v using val_ind''; unfold val_ref; auto.
+    repeat (split; auto).
+    induction H.
+    constructor.
+    constructor.
+    rewrite val_ref_eq; auto.
+    eapply IHForall.
   Qed.
 
-  Lemma val_ref_trans : Transitive val_ref.
+  Lemma val_ref_trans :
+    forall {v1 v2 v3},
+      val_ref v1 v2 ->
+      val_ref v2 v3 ->
+      val_ref v1 v3.
   Proof.
-    intros v1 v2 v3 H.
-    revert v3.
-    induction H; simpl; intros; inv H; auto.
-    - inv H1; auto.
-    - inv H1.
-      inv H5; auto.
-    - inv H1; auto.
+    intros v1.
+    induction v1 using val_ind''; intros v2 v3;
+      destruct v2; destruct v3; intros; simpl in *; eauto; try contradiction.
+    prog.
+    revert l l0 H3 H2.
+    induction vs; prog.
+    rewrite val_ref_eq in *.
+    eapply H2; eauto.
+    eapply IHvs; eauto.
   Qed.
 
-  Lemma V_val_ref {v1 v2} :
-    (forall i, V i v1 v2) ->
+  Lemma V_val_ref {i v1 v2} :
+    V i v1 v2 ->
     val_ref v1 v2.
   Proof.
-    revert v2.
-    induction v1 using val_ind'; intros; simpl.
-    - specialize (H 0).
-      destruct v2; simpl in *; try contradiction.
-      destruct H as [Hc Hlen]; subst.
-      symmetry in Hlen.
-      apply length_zero_iff_nil in Hlen; subst; auto.
-    - destruct v2.
-      + specialize (H 0); simpl in *; contradiction.
-      + destruct l0;
-          pose proof (H 1) as H1; simpl in *;
-          inv H1; subst;
-          inv H2.
-        clear H4 H6.
-
-        assert (HV' : forall i, V i v1 v /\ V i (Vconstr c l) (Vconstr c l0)).
-        {
-          intros.
-          specialize (H (S i)).
-          destruct i; simpl in *;
-            destruct H as [_ HFV];
-            inv HFV;
-            destruct v1; destruct v; try contradiction;
-            repeat (split; auto);
-            try (eapply Forall2_length; eauto);
-            try (eapply V_mono_Forall with (S i); eauto).
-        }
-
-        assert (HV0 : forall i, V i v1 v) by (intros; destruct (HV' i); auto).
-        assert (HV1 : forall i, V i (Vconstr c l) (Vconstr c l0)) by (intros; destruct (HV' i); auto).
-
-        auto.
-    - specialize (H 0); simpl in *.
-      destruct v2; try contradiction; auto.
-  Qed.
-
-  Lemma R_res_val_ref {v1 v2} :
-    (forall i, R i (Res v1) (Res v2)) ->
-    val_ref v1 v2.
-  Proof.
-    intros; eapply V_val_ref; eauto.
+    revert i v2.
+    induction v1 using val_ind''; prog.
+    - constructor.
+    - eapply val_ref_Vconstr; eauto.
+      generalize dependent l; induction vs; prog.
+      eapply H2; eauto.
   Qed.
 
   Lemma R_n_res_val_ref {n v1 v2} :
@@ -273,19 +297,19 @@ Section Refinement.
     remember (Res v2) as r2.
     generalize dependent v1.
     generalize dependent v2.
-    induction H; simpl; intros; subst.
-    - inv Heqr1; auto.
+    induction H; simpl; prog.
+    - inv Heqr1.
       apply val_ref_refl; auto.
     - pose proof (H 0) as HR0.
       destruct c2; simpl in HR0; try contradiction.
-      assert (Heqv : Res v = Res v) by auto.
+      apply V_val_ref in HR0.
       assert (Heqv2 : Res v2 = Res v2) by auto.
+      assert (Heqv : Res v = Res v) by auto.
       specialize (IHComp _ Heqv2 _ Heqv).
-      specialize (R_res_val_ref H); intros.
       eapply val_ref_trans; eauto.
   Qed.
 
-  (* Behavioral Refinement *)
+  (* Termination Refinement *)
   Theorem Top_n_val_ref n e1 e2 :
     Top_n n e1 e2 ->
     forall ρ1 ρ2,
@@ -297,9 +321,10 @@ Section Refinement.
           val_ref v1 v2.
   Proof.
     intros.
-    edestruct Top_n_adequacy with (ρ1 := ρ1) as [j2 [r2 [Hr2 HR]]]; eauto.
-    edestruct R_n_Res_inv as [v2 [Heq HVn]]; eauto; subst.
-    eexists; eexists; split; eauto.
+    edestruct Top_n_adequacy with (ρ1 := ρ1) as [j2 [r2 ?]]; eauto.
+    inv H2; prog.
+    edestruct R_n_Res_inv as [v2 ?]; eauto; prog.
+    eexists; eexists; prog; eauto.
     eapply R_n_res_val_ref; eauto.
   Qed.
 
@@ -311,23 +336,25 @@ Section Linking.
      1. e1 and e2 can contain multiple holes
      2. f can be either free or not in either e1 or e2 as long as e1 is compiled by the pipeline.
      3. x can be either free or not in e2 as long as e2 is compiled by the pipeline.
-     4. w needs to be exposed
+     4. w needs to be exposed *)
+  Definition link f x e1 e2 : exp :=
+    Efun f [] e1
+      (Eletapp x f [] e2).
 
-     Print link.
-   *)
-
+  (* Note the following lemma is not applicable as [trans_correct] is not the top-level relation.
+   * Thus, we need to show the compat lemmas for fun and letapp with [related_top] *)
   Lemma related_preserves_linking f x e1 e2 e1' e2':
     related e1 e2 ->
     related e1' e2' ->
     related (link f x e1 e1') (link f x e2 e2').
   Proof.
     unfold link.
-    intros He He'.
+    intros Hw He He'.
     eapply fun_compat; eauto.
     eapply letapp_compat; eauto.
   Qed.
 
-  (* [related] is strictly stronger than [related_top] *)
+  (* [related] is stronger than [related_top] due to [G_top] *)
   Lemma related_related_top e1 e2 :
     occurs_free e2 \subset occurs_free e1 ->
     related e1 e2 ->
@@ -340,51 +367,22 @@ Section Linking.
     eapply G_top_G; eauto.
   Qed.
 
-  Lemma related_top_related e1 e2 :
-    related_top e1 e2 ->
-    related e1 e2.
-  Proof.
-    unfold related_top, related.
-    intros.
-    destruct H as [HS H].
-    eapply H; eauto.
-  Abort.
-
   (* Environment Lemmas *)
-  Lemma G_top_get {i Γ ρ1 ρ2}:
-  G_top i Γ ρ1 ρ2 ->
-  forall x v1,
-    (x \in Γ) ->
-    M.get x ρ1 = Some v1 ->
-    exists v2,
-      M.get x ρ2 = Some v2 /\
-        V i v1 v2.
-  Proof.
-    unfold G_top.
-    intros HG; intros.
-    edestruct HG as [v1' [v2 [Heqv1 [Heqv2 HV]]]]; eauto; invc.
-    fcrush.
-  Qed.
-
   Lemma G_top_get_list {i Γ1 ρ1 ρ2} :
     G_top i Γ1 ρ1 ρ2 ->
-    forall xs vs1,
+    forall xs,
       (FromList xs) \subset Γ1 ->
-      get_list xs ρ1 = Some vs1 ->
-      exists vs2,
+      exists vs1 vs2,
+        get_list xs ρ1 = Some vs1 /\
         get_list xs ρ2 = Some vs2 /\
-          Forall2 (V i) vs1 vs2.
+        Forall2 (V i) vs1 vs2.
   Proof.
-    intros HG xs.
-    induction xs; simpl; intros.
-    - fcrush.
-    - destruct (ρ1 ! a) eqn:Heq1; try discriminate.
-      destruct (get_list xs ρ1) eqn:Heq3; try discriminate.
-      inv H0.
-      unfold Ensembles.Included, Ensembles.In in *.
-      edestruct (G_top_get HG) as [v2 [Heqv2 HV]]; eauto.
-      eapply (H a); fcrush.
-      edestruct IHxs as [vs2 [Heqvs2 Vvs]]; eauto; fcrush.
+    unfold G_top.
+    induction xs; prog; simpl.
+    - eexists; eexists; prog.
+    - edestruct H as [v1 [v2 ?]]; prog; eauto.
+      edestruct IHxs as [vs1 [vs2 ?]]; prog; eauto.
+      eexists; eexists; prog.
   Qed.
 
   Lemma G_top_set {i Γ1 ρ1 ρ2}:
@@ -394,12 +392,10 @@ Section Linking.
       G_top i (x |: Γ1) (M.set x v1 ρ1) (M.set x v2 ρ2).
   Proof.
     unfold G_top.
-    intros.
-    destruct (M.elt_eq x0 x); subst.
-    - repeat rewrite M.gss.
-      fcrush.
-    - repeat (rewrite M.gso; auto).
-      fcrush.
+    prog.
+    destruct (M.elt_eq x0 x); prog.
+    - eexists; eexists; prog.
+    - inv H1; prog.
   Qed.
 
   Lemma G_top_set_lists {i Γ1 ρ1 ρ2}:
@@ -410,23 +406,14 @@ Section Linking.
       set_lists xs vs2 ρ2 = Some ρ4 ->
       G_top i (FromList xs :|: Γ1) ρ3 ρ4.
   Proof.
+    unfold G_top.
     intros HG xs.
-    induction xs; simpl; intros.
-    - destruct vs1; try discriminate.
-      destruct vs2; try discriminate.
-      invc.
-      unfold G_top.
-      fcrush.
-    - destruct vs1; try discriminate.
-      destruct vs2; try discriminate.
-      destruct (set_lists xs vs1 ρ1) eqn:Heq1; try discriminate.
-      destruct (set_lists xs vs2 ρ2) eqn:Heq2; try discriminate.
-      inv H; invc.
-      eapply G_top_subset; eauto.
-      eapply G_top_set; eauto.
-      normalize_sets.
-      rewrite Union_assoc; eauto.
-      fcrush.
+    induction xs; prog.
+    - destruct (M.elt_eq x a); prog.
+      + eexists; eexists; prog.
+      + eapply IHxs; eauto; prog.
+        rewrite <- Union_assoc in H2.
+        inv H2; prog.
   Qed.
 
   (* Monotonicity Lemma *)
@@ -436,33 +423,31 @@ Section Linking.
     G_top j Γ1 ρ1 ρ2.
   Proof.
     unfold G_top.
-    intros.
-    edestruct H as [v1 [v2 [Heqv1 [Heqv2 HV]]]]; eauto.
-    eexists; eexists; repeat split; eauto.
-    apply V_mono with i; eauto.
+    prog.
+    edestruct H as [v1 [v2 ?]]; eauto; prog.
+    eexists; eexists; prog; eauto.
+    eapply V_mono; eauto; prog.
   Qed.
 
   (* Compatibility Lemmas *)
   Lemma Vfun_V e e' :
     related_top e e' ->
-    forall i f xs Γ1 ρ1 ρ2,
+    forall i f xs Γ1  ρ1 ρ2,
       G_top i Γ1 ρ1 ρ2 ->
       occurs_free e \subset (FromList xs :|: (f |: Γ1)) ->
       V i (Vfun f ρ1 xs e) (Vfun f ρ2 xs e').
   Proof.
     unfold related_top.
     intros [HS He] i.
-    induction i; simpl; intros; auto;
-      repeat (split; auto); intros.
-
-    apply (He (i - (i - j)) ρ3 ρ4); auto.
+    induction i; prog.
+    apply (He j ρ3 ρ4); prog.
     eapply G_top_subset with (Γ1 := FromList xs :|: (f |: Γ1)); eauto.
     eapply G_top_set_lists; eauto.
-    eapply G_top_set; eauto.
-    eapply G_top_mono; eauto; try lia.
-    apply V_mono with i; try lia.
+    eapply G_top_set; eauto; try (prog; fail).
+    eapply G_top_mono; eauto; prog.
+    eapply V_mono with i; try lia.
     eapply IHi; eauto.
-    apply G_top_mono with (S i); eauto; lia.
+    eapply G_top_mono; eauto; prog.
   Qed.
 
   Lemma fun_compat_top e e' k k' f xs :
@@ -471,70 +456,75 @@ Section Linking.
     related_top (Efun f xs e k) (Efun f xs e' k').
   Proof.
     unfold related_top, E, E'.
-    intros [HSe He] [HSk Hk].
-    split; intros.
-    eapply free_fun_compat; eauto.
-
-    pose proof H as HG.
-    inv H1.
-    - fcrush.
-    - inv H2.
-      edestruct (Hk (i - 1) (M.set f (Vfun f ρ1 xs e) ρ1) (M.set f (Vfun f ρ2 xs e') ρ2)) with (j1 := c) (r1 := r1) as [j2 [r2 [Hk2 Rr]]]; eauto; try lia.
-      + eapply G_top_subset with (Γ1 := (f |: (occurs_free (Efun f xs e k)))); eauto.
-        * eapply G_top_set; eauto.
-          eapply G_top_mono; eauto; try lia.
-          eapply Vfun_V with (Γ1 := (occurs_free (Efun f xs e k))); eauto.
-          -- unfold related_top.
-             split; auto.
-          -- eapply G_top_mono; eauto; try lia.
-          -- eapply free_fun_e_subset; eauto.
-        * eapply free_fun_k_subset; eauto.
-      + exists (S j2), r2; split; auto.
-        apply R_mono with ((i - 1) - c); try lia; auto.
+    prog.
+    {
+      unfold Ensembles.Included, Ensembles.In in *; prog.
+      inv H3; prog.
+    }
+    pose proof H4 as HG; unfold G_top in HG; prog.
+    inv H5; prog.
+    - exists 0, OOT; prog.
+    - edestruct (H1 (i - 1) (M.set f (Vfun f ρ1 xs e) ρ1) (M.set f (Vfun f ρ2 xs e') ρ2)) with (j1 := c) (r1 := r1) as [j2 [r2 ?]]; eauto; try lia.
+      + eapply G_top_subset with (Γ1 := (f |: (occurs_free (Efun f xs e k)))).
+        eapply G_top_set; eauto; try (prog; fail).
+        eapply G_top_mono; eauto; try lia.
+        eapply Vfun_V with (Γ1 := (occurs_free (Efun f xs e k))); eauto; prog.
+        unfold related_top; prog.
+        eapply G_top_mono; eauto; try lia.
+        eapply free_fun_e_subset; eauto.
+        eapply free_fun_k_subset; eauto.
+      + fcrush.
+      + exists (S j2), r2.
+        inv H5.
+        split.
+        fcrush.
+        eapply R_mono; eauto; prog.
   Qed.
 
   Lemma letapp_compat_top k k' xs x f :
     related_top k k' ->
     related_top (Eletapp x f xs k) (Eletapp x f xs k').
   Proof.
-    unfold related_top, E, E'.
-    intros [HSk Hk].
-    split; intros.
-    eapply free_letapp_compat; eauto.
+    unfold related_top, E, E', R, R'.
+    prog.
+    {
+      unfold Ensembles.Included, Ensembles.In in *; prog.
+      inv H1; auto.
+    }
 
-    pose proof H as HG.
-    inv H1.
+    pose proof H1 as HG; unfold G_top in HG; prog.
+    inv H3.
     - fcrush.
-    - inv H2.
-      2 : { fcrush. }
-      edestruct (G_top_get HG f) as [fv2 [Heqfv2 HVf]]; eauto.
-      destruct fv2.
-      2 : { destruct i; fcrush. }
-      destruct i.
-      fcrush.
-      simpl in HVf.
-      destruct HVf as [Hlen HV].
-
-      edestruct (G_top_get_list HG xs) as [vs2 [Heqvs2 HVvs]]; eauto.
-      eapply free_letapp_xs_subset; eauto.
-
-      destruct (set_lists_length3 (M.set v0 (Vfun v0 t l e0) t) l vs2) as [ρ4 Heqρ4].
-      rewrite <- (Forall2_length _ _ _ HVvs).
-      rewrite <- (set_lists_length_eq _ _ _ _ H10); auto.
-
-      unfold E' in HV.
-      edestruct (HV i vs vs2 ρ'' ρ4) with (j1 := c0) as [j2 [r2 [He0 HR]]]; eauto; try lia.
+    - inv H4.
+      edestruct (HG f) as [v1 [v2 ?]]; eauto; prog.
+      edestruct (G_top_get_list H1 xs) as [vs1 [vs2 ?]]; prog.
+      eapply free_letapp_xs_subset.
+      destruct (set_lists_length3 (M.set v0 (Vfun v0 t l e0) t) l vs2) as [ρ4 ?].
+      {
+        rewrite <- (Forall2_length _ _ _ H10).
+        rewrite <- (set_lists_length_eq _ _ _ _ H12); auto.
+      }
+      unfold E, E' in *.
+      destruct i; prog.
+      edestruct (H5 i vs1 vs2 ρ'' ρ4) with (j1 := c0) as [j2 [r2 ?]]; eauto.
       + eapply V_mono_Forall; eauto; lia.
-      + destruct r2; simpl in HR; try contradiction.
-        edestruct (Hk (i - c0) (M.set x v ρ1) (M.set x v1 ρ2)) with (j1 := c') as [j3 [r3 [He1 HR']]]; eauto; try lia.
-        eapply G_top_subset with (Γ1 := x |: (occurs_free (Eletapp x f xs k))); eauto.
-        eapply G_top_set; eauto.
-        eapply G_top_mono; eauto; lia.
-
-        * eapply V_mono; eauto; try lia.
-        * eapply free_letapp_k_subset; eauto.
-        * exists (S (j2 + j3)), r3; split; eauto.
-          eapply R_mono; eauto; lia.
+      + lia.
+      + prog.
+        destruct r2; try contradiction.
+        edestruct (H0 (i - c0) (M.set x v ρ1) (M.set x v1 ρ2)) with (j1 := c') as [j3 [r3 ?]]; eauto.
+        * eapply G_top_subset with (Γ1 := x |: (occurs_free (Eletapp x f xs k))); eauto; prog.
+          eapply G_top_set; eauto; prog.
+          eapply G_top_mono; eauto; lia.
+          eapply free_letapp_k_subset.
+        * lia.
+        * inv H16.
+          destruct r1; destruct r3; try contradiction.
+          fcrush.
+          exists (S (j2 + j3)), (Res v3).
+          split.
+          fcrush.
+          eapply V_mono; eauto; prog.
+      + fcrush.
   Qed.
 
   (* Linking Preservation for [related_top] *)
