theories/LambdaANF/ReflLex.v
@@ -1,0 +1,766 @@
+From Coq Require Import ZArith.ZArith Sets.Ensembles Lists.List Classes.RelationClasses.
+From compcert.lib Require Export Maps.
+From CertiCoq.LambdaANF Require Import Ensembles_util map_util set_util List_util tactics.
+From CertiCoq.Libraries Require Import maps_util.
+Import ListNotations.
+Require Import Lia.
+From Hammer Require Import Hammer Tactics Reflect.
+
+From Common Require Import Util.
+From LambdaANF Require Import Util Tactics ANF ANFLex.
+
+(* Logical Relations *)
+Definition R' (P : nat -> val -> val -> Prop) (i : nat) (r1 : res) (r2 : res) :=
+  match r1, r2 with
+  | OOT, OOT => True
+  | Res v1, Res v2 => P i v1 v2
+  | _, _ => False
+  end.
+
+Definition E' (P : nat -> val -> val -> Prop) (i : nat) (ρ1 : env) (e1 :exp) (ρ2 : env) (e2 : exp) : Prop :=
+  forall j1 r1,
+    j1 <= i ->
+    bstep_fuel ρ1 e1 j1 r1 ->
+    exists j2 r2,
+      bstep_fuel ρ2 e2 j2 r2 /\
+      R' P (i - j1) r1 r2.
+
+Fixpoint V (i : nat) (v1 : val) (v2 : val) {struct i} : Prop :=
+  let fix V' (v1 : val) (v2 : val) {struct v1} : Prop :=
+  match v1, v2 with
+  | Vconstr c1 vs1, Vconstr c2 vs2 =>
+      let fix Forall2_aux vs1 vs2 :=
+        match vs1, vs2 with
+        | [], [] => True
+        | v1 :: vs1, v2 :: vs2 =>
+            V' v1 v2 /\ Forall2_aux vs1 vs2
+        | _, _ => False
+        end in
+      c1 = c2 /\
+      Forall2_aux vs1 vs2
+
+  | Vfun f1 ρ1 xs1 e1, Vfun f2 ρ2 xs2 e2 =>
+      length xs1 = length xs2 /\
+      forall j vs1 vs2 ρ3 ρ4,
+        set_lists xs1 vs1 (M.set f1 (Vfun f1 ρ1 xs1 e1) ρ1) = Some ρ3 ->
+        set_lists xs2 vs2 (M.set f2 (Vfun f2 ρ2 xs2 e2) ρ2) = Some ρ4 ->
+        match i with
+        | 0 => True
+        | S i0 =>
+            j <= i0 ->
+            Forall2 (V (i0 - (i0 - j))) vs1 vs2 ->
+            E' V (i0 - (i0 - j)) ρ3 e1 ρ4 e2
+        end
+
+  | _, _ => False
+  end in
+  V' v1 v2.
+
+Definition V' (i : nat) (v1 : val) (v2 : val) : Prop :=
+  match v1, v2 with
+  | Vconstr c1 vs1, Vconstr c2 vs2 =>
+      c1 = c2 /\ Forall2 (V i) vs1 vs2
+
+  | Vfun f1 ρ1 xs1 e1, Vfun f2 ρ2 xs2 e2 =>
+      length xs1 = length xs2 /\
+      forall j vs1 vs2 ρ3 ρ4,
+        set_lists xs1 vs1 (M.set f1 (Vfun f1 ρ1 xs1 e1) ρ1) = Some ρ3 ->
+        set_lists xs2 vs2 (M.set f2 (Vfun f2 ρ2 xs2 e2) ρ2) = Some ρ4 ->
+        j < i ->
+        Forall2 (V j) vs1 vs2 ->
+        E' V j ρ3 e1 ρ4 e2
+  | _, _ => False
+  end.
+
+Lemma V_eq (i : nat) (v1 v2 : val) :
+  V i v1 v2 <-> V' i v1 v2.
+Proof.
+  destruct v1; destruct v2; prog;
+  unfold V' in *; try (destruct i; simpl in *; prog; split; prog; fail).
+  - destruct i; simpl in *; split; prog.
+    + specialize (H0 j); rewrite normalize_step in *; try lia.
+      eapply H0; try lia; eauto.
+    + specialize (H0 j); rewrite normalize_step in *; try lia.
+      eapply H0; try lia; eauto.
+  - destruct i; simpl in *; split; prog.
+    + generalize dependent l0.
+      induction l; destruct l0; prog.
+    + generalize dependent l0.
+      induction l; destruct l0; prog.
+      apply IHl; auto.
+    + generalize dependent l0.
+      induction l; destruct l0; prog.
+    + generalize dependent l0.
+      induction l; destruct l0; prog.
+      apply IHl; auto.
+Qed.
+
+(* Disallow unfolding V. Always use V_eq to turn it into V' *)
+Opaque V.
+Arguments V : simpl never.
+
+Notation R := (R' V).
+
+Notation E := (E' V).
+
+Hint Extern 1 =>
+       (match goal with
+        | [H : V _ (Vconstr _ _) _ |- _] => rewrite V_eq in H; unfold V' in H
+        | [H : V _ _ (Vconstr _ _) |- _] => rewrite V_eq in H; unfold V' in H
+        | [H : V _ (Vfun _ _ _ _) _ |- _] => rewrite V_eq in H; unfold V' in H
+        | [H : V _ _ (Vfun _ _ _ _) |- _] => rewrite V_eq in H; unfold V' in H
+        | [ |- V _ (Vconstr _ _) _ ] => rewrite V_eq; unfold V'
+        | [ |- V _ _ (Vconstr _ _) ] => rewrite V_eq; unfold V'
+        | [ |- V _ (Vfun _ _ _ _) _] => rewrite V_eq; unfold V'
+        | [ |- V _ _ (Vfun _ _ _ _)] => rewrite V_eq; unfold V'
+        | [ |- R _ OOT _] => simpl
+        | [ |- R _ _ OOT] => simpl
+        | [ H : R _ OOT _ |- _] => simpl in H
+        | [ H : R _ _ OOT |- _] => unfold R, R' in H
+        | [ |- R _ (Res _) _] => simpl
+        | [ |- R _ _ (Res _)] => simpl
+        | [ H : R _ (Res _) _ |- _] => simpl in H
+        | [ H : R _ _ (Res _) |- _] => unfold R, R' in H
+        end; shelve) : custom_automation.
+
+(* Environment Relation *)
+Definition G i Γ ρ1 ρ2 :=
+  forall x,
+    (x \in Γ) ->
+    forall v1,
+      M.get x ρ1 = Some v1 ->
+      exists v2,
+        M.get x ρ2 = Some v2 /\
+        V i v1 v2.
+
+Definition related e1 e2 :=
+  forall i ρ1 ρ2,
+    G i (occurs_free e1) ρ1 ρ2 ->
+    E i ρ1 e1 ρ2 e2.
+
+(* Environment Lemmas *)
+Lemma G_set {i Γ ρ1 ρ2}:
+  G i Γ ρ1 ρ2 ->
+  forall {x v1 v2},
+    V i v1 v2 ->
+    G i (x |: Γ) (M.set x v1 ρ1) (M.set x v2 ρ2).
+Proof.
+  intros HG; prog.
+  intro.
+  destruct (M.elt_eq x0 x); prog.
+  - eexists; eauto; prog.
+  - inv H0; prog.
+Qed.
+
+Lemma G_set_lists {i Γ ρ1 ρ2}:
+  G i Γ ρ1 ρ2 ->
+  forall {xs vs1 vs2 ρ3 ρ4},
+    Forall2 (V i) vs1 vs2 ->
+    set_lists xs vs1 ρ1 = Some ρ3 ->
+    set_lists xs vs2 ρ2 = Some ρ4 ->
+    G i (FromList xs :|: Γ) ρ3 ρ4.
+Proof.
+  unfold G.
+  intros HG xs.
+  induction xs; simpl; intros.
+  - destruct vs1; try discriminate.
+    destruct vs2; try discriminate.
+    inv H0; inv H1.
+    eapply HG; eauto.
+    prog.
+  - destruct vs1; try discriminate.
+    destruct vs2; try discriminate.
+    destruct (set_lists xs vs1 ρ1) eqn:Heq1; try discriminate.
+    destruct (set_lists xs vs2 ρ2) eqn:Heq2; try discriminate.
+    inv H; inv H0; inv H1.
+    destruct (M.elt_eq x a); prog.
+    + eexists; prog.
+    + eapply IHxs; eauto.
+      rewrite <- Union_assoc in H2.
+      inv H2; prog.
+Qed.
+
+Lemma G_get {i Γ ρ1 ρ2 x v1}:
+  G i Γ ρ1 ρ2 ->
+  M.get x ρ1 = Some v1 ->
+  (x \in Γ) ->
+  exists v2,
+    M.get x ρ2 = Some v2 /\
+    V i v1 v2.
+Proof.
+  unfold G; prog.
+Qed.
+
+Lemma G_get_list {i Γ ρ1 ρ2 xs vs1} :
+  G i Γ ρ1 ρ2 ->
+  get_list xs ρ1 = Some vs1 ->
+  (FromList xs \subset Γ) ->
+  exists vs2,
+    get_list xs ρ2 = Some vs2 /\
+    Forall2 (V i) vs1 vs2.
+Proof.
+  unfold G.
+  intros HG H_get_list H_subset.
+  revert vs1 H_get_list.
+  induction xs; prog; simpl.
+  - eexists; prog.
+  - edestruct HG as [v2 ?]; eauto; prog.
+    edestruct IHxs as [vs2 ?]; eauto.
+    eexists; prog.
+Qed.
+
+(* Monotonicity Lemmas *)
+Lemma V_mono i :
+  forall {j v1 v2},
+    V i v1 v2 ->
+    j <= i ->
+    V j v1 v2.
+Proof.
+  intros.
+  generalize dependent v2.
+  induction v1 using val_ind''; prog.
+  - eapply H1; eauto; prog.
+  - generalize dependent l.
+    induction vs; prog.
+Qed.
+
+Lemma V_mono_Forall {vs1 vs2} i j :
+  Forall2 (V i) vs1 vs2 ->
+  j <= i ->
+  Forall2 (V j) vs1 vs2.
+Proof.
+  intros H.
+  revert j.
+  induction H; simpl; intros; auto.
+  constructor; eauto.
+  eapply V_mono; eauto.
+Qed.
+
+Lemma R_mono {r1 r2} i j :
+  R i r1 r2 ->
+  j <= i ->
+  R j r1 r2.
+Proof.
+  unfold R.
+  intros.
+  destruct r1; auto.
+  destruct r2; auto.
+  eapply V_mono; eauto.
+Qed.
+
+Lemma E_mono {ρ1 ρ2 e1 e2} i j:
+  E i ρ1 e1 ρ2 e2 ->
+  j <= i ->
+  E j ρ1 e1 ρ2 e2.
+Proof.
+  unfold E.
+  intros.
+  destruct (H j1 r1) as [j2 [r2 [Hr2 HR]]]; auto; try lia.
+  exists j2, r2; split; eauto.
+  apply R_mono with (i - j1); try lia; auto.
+Qed.
+
+Lemma G_mono {Γ ρ1 ρ2} i j:
+  G i Γ ρ1 ρ2 ->
+  j <= i ->
+  G j Γ ρ1 ρ2.
+Proof.
+  unfold G.
+  intros.
+  edestruct H as [v2 [Heqv2 Vv]]; eauto.
+  exists v2; split; auto.
+  apply V_mono with i; eauto.
+Qed.
+
+Lemma G_subset Γ1 Γ2 i ρ1 ρ2:
+  G i Γ1 ρ1 ρ2 ->
+  Γ2 \subset Γ1 ->
+  G i Γ2 ρ1 ρ2.
+Proof.
+  unfold G.
+  intros.
+  eapply H; prog.
+Qed.
+
+(* Compatibility Lemmas *)
+Lemma ret_compat x :
+  related (Eret x) (Eret x).
+Proof.
+  unfold related, E, E'.
+  intros.
+  inv H1; prog.
+  - exists 0; eexists; prog; eauto.
+  - inv H2.
+    edestruct (G_get H H3) as [v2 ?]; eauto; prog.
+    eexists (S _); eexists (Res _); prog; eauto; prog.
+    eapply V_mono; eauto; prog.
+Qed.
+
+Lemma constr_compat {k} x t xs :
+  related k k ->
+  related (Econstr x t xs k) (Econstr x t xs k).
+Proof.
+  unfold related, E, E'.
+  intros.
+  inv H2; prog.
+  - exists 0; eexists; prog.
+  - inv H3.
+    destruct (G_get_list H0 H9) as [vs' ?]; prog.
+    eapply free_constr_xs_subset.
+    assert (length vs = length vs').
+    {
+      rewrite <- (get_list_length_eq _ _ _ H9).
+      rewrite <- (get_list_length_eq _ _ _ H2); auto.
+    }
+
+    edestruct (H i (M.set x (Vconstr t vs) ρ1) (M.set x (Vconstr t vs') ρ2)) with (j1 := c) as [j2 [r2 ?]]; eauto; prog.
+    + eapply G_subset; eauto.
+      eapply G_set; prog.
+      eauto.
+      eapply free_constr_k_subset.
+    + eexists (S _); exists r2; prog; eauto; prog.
+      eapply R_mono; try exact H6; prog.
+Qed.
+
+Lemma Vfun_V {e e'} :
+  related e e' ->
+  forall {i Γ ρ1 ρ2} f xs,
+    G i Γ ρ1 ρ2 ->
+    (occurs_free e) \subset (FromList xs :|: (f |: Γ)) ->
+    V i (Vfun f ρ1 xs e) (Vfun f ρ2 xs e').
+Proof.
+  unfold related.
+  intros He i.
+  induction i; prog.
+  eapply He.
+  eapply G_subset; eauto.
+  eapply G_set_lists; eauto.
+  apply G_set.
+  - apply G_mono with (S i); auto; lia.
+  - apply V_mono with i; try lia.
+    eapply IHi; eauto.
+    apply G_mono with (S i); auto; lia.
+Qed.
+
+Lemma fun_compat {e k e' k'} f xs :
+  related e e' ->
+  related k k' ->
+  related (Efun f xs e k) (Efun f xs e' k').
+Proof.
+  unfold related, E, E'.
+  intros.
+  inv H3.
+  - exists 0; eexists; prog.
+  - edestruct (H0 (i - 1) (M.set f (Vfun f ρ1 xs e) ρ1) (M.set f (Vfun f ρ2 xs e') ρ2)) with (j1 := c) (r1 := r1) as [j2 [r2 ?]]; eauto; try lia.
+    + eapply G_subset; eauto.
+      eapply G_set; eauto.
+      * eapply G_mono with i; eauto; lia.
+      * eapply Vfun_V; eauto; prog.
+        eapply G_mono; eauto; prog.
+        eapply free_fun_e_subset.
+      * eapply free_fun_k_subset.
+    + inv H4.
+      prog.
+    + eexists (S _), r2; prog; eauto.
+      eapply R_mono; eauto; prog.
+Qed.
+
+Lemma app_compat f xs :
+  related (Eapp f xs) (Eapp f xs).
+Proof.
+  unfold related, E, E'.
+  intros.
+  inv H1.
+  - exists 0; eexists; prog.
+  - inv H2.
+    edestruct (G_get H H4) as [v2 ?]; eauto; prog.
+    (* destruct i; prog. *)
+    destruct (G_get_list H H5) as [vs2 ?]; eauto; prog.
+    eapply free_app_xs_subset.
+    destruct (set_lists_length3 (M.set v (Vfun v t l e0) t) l vs2) as [ρ4 ?].
+    {
+    rewrite <- (Forall2_length _ _ _ H8).
+    rewrite <- (set_lists_length_eq _ _ _ _ H6).
+    erewrite eq_sym; eauto.
+    }
+
+    assert (HE : E (i - 1) ρ'' e ρ4 e0).
+    {
+      eapply (H3 (i - 1) vs vs2); eauto; prog.
+      eapply V_mono_Forall; eauto; prog.
+    }
+
+    unfold E, E' in HE.
+    edestruct (HE c r1) as [j2 [r2 ?]]; eauto; prog.
+    exists (S j2), r2; prog; eauto; prog.
+    eapply R_mono; eauto; prog.
+Qed.
+
+Lemma proj_compat x i y e e':
+  related e e' ->
+  related (Eproj x i y e) (Eproj x i y e').
+Proof.
+  unfold related, E, E'.
+  intros.
+  inv H2.
+  - exists 0; eexists; prog.
+  - inv H3.
+    edestruct (G_get H0 H9) as [v2 ?]; eauto; prog.
+    rename l into vs'.
+    destruct (Forall2_nth_error H10 H4) as [v' ?]; prog.
+    edestruct (H i0 (M.set x v ρ1) (M.set x v' ρ2)) with (j1 := c) as [j2 [r2 [He' HR]]]; eauto; try lia.
+    + eapply G_subset; eauto.
+      eapply G_set; eauto; prog.
+      eapply free_proj_k_subset.
+    + exists (S j2), r2; prog; eauto; prog.
+      eapply R_mono; eauto; prog.
+Qed.
+
+Lemma letapp_compat {k k'} x f xs :
+  related k k' ->
+  related (Eletapp x f xs k) (Eletapp x f xs k').
+Proof.
+  intros.
+  specialize (app_compat f xs); intros Ha.
+  unfold related, E, E' in *.
+  intros.
+  assert (HGa : G i (occurs_free (Eapp f xs)) ρ1 ρ2).
+  {
+    eapply G_subset; eauto; prog.
+    intro; intros.
+    inv H3.
+    - eapply Free_letapp2.
+    - eapply Free_letapp3; auto.
+  }
+  specialize (Ha _ _ _ HGa).
+  inv H2.
+  - exists 0; eexists; prog.
+  - inv H3.
+    destruct (Ha (S c0) (Res v)) as [j1 [ra [Hbstep HR]]]; try lia; eauto.
+    prog.
+    destruct ra; try contradiction.
+    edestruct (H (i - (S c0)) (M.set x v ρ1) (M.set x v0 ρ2)) with (j1 := c') as [j2 [r2 ?]]; eauto; try lia; prog.
+    + eapply (G_subset (x |: occurs_free (Eletapp x f xs k))); eauto.
+      eapply G_set; prog.
+      eapply G_mono; eauto; prog.
+      eapply free_letapp_k_subset.
+    + exists (j1 + j2), r2; split.
+      ++ inv Hbstep.
+         inv H4.
+         rewrite_math ((S c + j2) = S (c + j2)); eauto.
+      ++ eapply R_mono; eauto; prog.
+    + eexists; eexists; split; eauto.
+      unfold R; simpl; auto.
+Qed.
+
+Lemma case_nil_compat x:
+  related (Ecase x []) (Ecase x []).
+Proof.
+  unfold related, G, E, E', R'.
+  prog.
+  inv H1; fcrush.
+Qed.
+
+Lemma case_cons_compat e e' x cl cl' c:
+  related e e' ->
+  related (Ecase x cl) (Ecase x cl') ->
+  related (Ecase x ((c, e) :: cl)) (Ecase x ((c, e') :: cl')).
+Proof.
+  unfold related, E, E'.
+  prog.
+  inv H3.
+  - fcrush.
+  - inv H4.
+    edestruct (G_get H1 H6) as [v2 ?]; eauto; prog.
+    inv H7.
+    + edestruct (H i ρ1 ρ2) with (j1 := c0) as [j2 [r2 ?]]; eauto; prog.
+      eapply G_subset; eauto; prog.
+      eapply free_case_hd_subset.
+      exists (S j2), r2; prog; eauto; prog.
+      eapply R_mono; eauto; prog.
+    + edestruct (H0 i ρ1 ρ2) with (j1 := S c0) (r1 := r1) as [j2 [r2 ?]]; eauto; prog; eauto.
+      eapply G_subset; eauto; prog.
+      eapply free_case_tl_subset.
+      destruct j2.
+      * fcrush.
+      * exists (S j2); eexists.
+        split; eauto.
+        econstructor; eauto.
+        inv H4.
+        inv H11.
+        econstructor; eauto.
+        econstructor; eauto.
+        prog.
+Qed.
+
+(* Fundamental Property *)
+Lemma fundamental_property e :
+  related e e.
+Proof.
+  induction e using exp_ind'.
+  - apply ret_compat.
+  - apply app_compat.
+  - apply fun_compat; auto.
+  - apply letapp_compat; auto.
+  - apply constr_compat; auto.
+  - apply case_nil_compat; auto.
+  - apply case_cons_compat; auto.
+  - apply proj_compat; auto.
+Qed.
+
+(* Reflexivity *)
+Lemma refl_V_G :
+  forall i,
+    (forall k : nat, k < S i -> forall v : val, V k v v) ->
+    forall ρ,
+      forall xs Γ j vs1 vs2 ρ1 ρ2,
+        j <= i ->
+        Forall2 (V j) vs1 vs2 ->
+        set_lists xs vs1 ρ = Some ρ1 ->
+        set_lists xs vs2 ρ = Some ρ2 ->
+        G j Γ ρ1 ρ2.
+Proof.
+  unfold G.
+  intros i HI ρ xs.
+  induction xs; prog.
+  - eexists; prog; eauto.
+    eapply HI; prog.
+  - destruct (M.elt_eq x a); prog.
+    + eexists; prog.
+    + edestruct IHxs as [v2 ?]; eauto; prog.
+Qed.
+
+Lemma refl_V_ForallV :
+  forall i,
+    (forall k : nat, k < S i -> forall v : val, V k v v) ->
+    forall vs j,
+      j <= i ->
+      Forall2 (V j) vs vs.
+Proof.
+  intros i HI vs.
+  induction vs; simpl; prog.
+  eapply HI; eauto; try lia.
+Qed.
+
+Theorem refl_V :
+  forall i v, V i v v.
+Proof.
+  intros i.
+  induction i using lt_wf_rec.
+  induction v using val_ind''; prog.
+  - eapply fundamental_property.
+    eapply refl_V_G with (ρ := (M.set f (Vfun f ρ xs e) ρ)); eauto.
+    intros.
+    eapply H; prog.
+  - induction vs; prog.
+Qed.
+
+Corollary refl_V_Forall vs :
+  forall i, Forall2 (V i) vs vs.
+Proof.
+  intros i.
+  induction vs; prog.
+  eapply refl_V; prog.
+Qed.
+
+Theorem refl_R :
+  forall i r, R i r r.
+Proof.
+  unfold R'.
+  intros.
+  destruct r; auto.
+  apply refl_V; auto.
+Qed.
+
+Theorem refl_E :
+  forall i ρ e, E i ρ e ρ e.
+Proof.
+  unfold E, E'.
+  intros.
+  exists j1, r1; prog.
+  apply refl_R; auto.
+Qed.
+
+Theorem refl_G :
+  forall i Γ ρ, G i Γ ρ ρ.
+Proof.
+  unfold G.
+  intros.
+  eexists; split; eauto.
+  apply refl_V.
+Qed.
+
+(* Transitivity of E *)
+Lemma trans_E_aux i :
+  (forall m : nat,
+      m <= i ->
+      forall v1 v2 v3 : val,
+        V m v1 v2 ->
+        (forall i : nat, V i v2 v3) ->
+        V m v1 v3) ->
+  forall {ρ1 e1 ρ2 e2 ρ3 e3},
+    E i ρ1 e1 ρ2 e2 ->
+    (forall i, E i ρ2 e2 ρ3 e3) ->
+    E i ρ1 e1 ρ3 e3.
+Proof.
+  unfold E, E'.
+  intros IH; intros.
+  edestruct H as [j2 [r2 [Hr2 HR]]]; eauto.
+  edestruct (H0 j2) as [j3 [r3 [Hr3 HR']]]; eauto; try lia.
+  eexists; eexists; split; eauto.
+  unfold R' in *.
+  destruct r1; destruct r2; destruct r3; try contradiction; auto.
+  eapply IH; eauto; try lia.
+  intros.
+  edestruct (H0 (i0 + j2) j2) as [j3' [r3' [Hr3' HR'']]]; eauto; try lia.
+  simpl in *.
+  destruct r3'; try contradiction.
+  edestruct (bstep_fuel_deterministic v1 v2 Hr3 Hr3'); eauto; subst.
+  eapply V_mono; eauto; try lia.
+Qed.
+
+Lemma trans_V_Forall_aux i :
+  (forall m : nat,
+      m <= i ->
+      forall v1 v2 v3 : val,
+        V m v1 v2 ->
+        (forall i : nat, V i v2 v3) ->
+        V m v1 v3) ->
+  forall {vs1},
+    forall {vs2 vs3},
+      Forall2 (V i) vs1 vs2 ->
+      (forall i, Forall2 (V i) vs2 vs3) ->
+      Forall2 (V i) vs1 vs3.
+Proof.
+  intros IH vs1.
+  induction vs1; simpl; intros.
+  - inv H.
+    eapply H0; eauto.
+  - inv H.
+    pose proof (H0 i) as H2'.
+    inv H2'.
+    constructor.
+    + eapply IH; eauto; try lia.
+      intros.
+      specialize (H0 i0).
+      inv H0; auto.
+    + eapply IHvs1; eauto; try lia.
+      intros.
+      specialize (H0 i0).
+      inv H0; auto.
+Qed.
+
+Theorem trans_V :
+  forall {i v1 v2 v3},
+    V i v1 v2 ->
+    (forall i, V i v2 v3) ->
+    V i v1 v3.
+Proof.
+  intros i.
+  induction i using lt_wf_rec1.
+  induction v1 using val_ind''; prog.
+  - pose proof (H1 i); prog.
+    assert (length l = length vs2) by (rewrite H3; eapply set_lists_length_eq; eauto).
+    destruct (set_lists_length3 (M.set v (Vfun v t l e0) t) _ _ H9) as [ρ5 ?].
+
+    assert (length vs2 = length vs1) by (eapply eq_sym; eapply Forall2_length; eauto).
+    edestruct (set_lists_length _ (M.set v (Vfun v t l e0) t) _ _ _ _ H11 H6) as [ρ6 ?].
+
+    eapply trans_E_aux; eauto.
+    + prog.
+      eapply H; eauto; prog.
+    + intro i0.
+      specialize (H1 (S i0)); prog.
+      specialize (H13 i0 vs2 vs2).
+      eapply H13; eauto; prog.
+      eapply refl_V_Forall; prog.
+  - pose proof (H2 i); prog.
+    (* clear H1 H3 H4 H5. *)
+    generalize dependent l0.
+    generalize dependent l.
+    revert H0.
+    induction vs; prog.
+    + eapply H6; eauto; prog.
+      specialize (H2 i0); prog.
+    + eapply IHvs; eauto; prog.
+      specialize (H2 i0); prog.
+Qed.
+
+Corollary trans_R {i r1 r2 r3} :
+  R i r1 r2 ->
+  (forall k, R k r2 r3) ->
+  R i r1 r3.
+Proof.
+  unfold R, R'.
+  intros.
+  destruct r1; destruct r2; destruct r3; prog.
+  eapply trans_V; eauto.
+Qed.
+
+Corollary trans_E {i ρ1 e1 ρ2 e2 ρ3 e3}:
+  E i ρ1 e1 ρ2 e2 ->
+  (forall i, E i ρ2 e2 ρ3 e3) ->
+  E i ρ1 e1 ρ3 e3.
+Proof.
+  intros.
+  eapply trans_E_aux; eauto.
+  intros.
+  eapply trans_V; eauto.
+Qed.
+
+(* Top Level *)
+Definition G_top i Γ1 ρ1 ρ2 :=
+  forall x,
+    (x \in Γ1) ->
+    exists v1 v2,
+      M.get x ρ1 = Some v1 /\
+      M.get x ρ2 = Some v2 /\
+      V i v1 v2.
+
+Lemma G_top_G : forall {i Γ1 ρ1 ρ2},
+    G_top i Γ1 ρ1 ρ2 ->
+    G i Γ1 ρ1 ρ2.
+Proof.
+  unfold G_top, G; prog.
+  unfold Ensembles.Included, Ensembles.In, Dom_map in *; prog.
+  edestruct H as [v1' [v2 ?]]; eauto; prog.
+  eexists; prog; eauto.
+Qed.
+
+Definition related_top etop etop' :=
+  occurs_free etop' \subset occurs_free etop /\
+  forall i ρ1 ρ2,
+    G_top i (occurs_free etop) ρ1 ρ2 ->
+    E i ρ1 etop ρ2 etop'.
+
+Theorem top etop:
+  related_top etop etop.
+Proof.
+  unfold related_top; prog.
+  eapply fundamental_property.
+  eapply G_top_G; eauto.
+Qed.
+
+(* Reflexivity of [related_top] *)
+Corollary refl_related_top :
+  Reflexive related_top.
+Proof.
+  unfold related_top, Reflexive; prog.
+  eapply fundamental_property.
+  eapply G_top_G; eauto.
+Qed.
+
+(* Transitivity of [related_top] *)
+Theorem trans_related_top :
+  Transitive related_top.
+Proof.
+  intros e1 e2 e3.
+  unfold related_top, G_top; prog.
+  - eapply Included_trans; eauto.
+  - eapply trans_E; eauto; prog.
+    unfold Ensembles.Included, Ensembles.In in *.
+    eapply H1; prog.
+    edestruct H3 as [v1 [v2 ?]]; eauto; prog.
+    eexists; eexists; prog; eauto; prog.
+    eapply refl_V; prog.
+Qed.
