theories/LambdaANF/Util.v
@@ -1,0 +1,459 @@
+From Coq Require Import Sets.Ensembles Lists.List.
+From compcert.lib Require Export Maps.
+From CertiCoq.Libraries Require Import maps_util.
+From CertiCoq.LambdaANF Require Import Ensembles_util map_util tactics.
+From CertiCoq.Libraries Require Import maps_util.
+Import ListNotations.
+Require Import Lia.
+
+Lemma normalize_step : forall i j, j <= i -> i - (i - j) = j.
+Proof. intros; lia. Qed.
+
+Lemma Forall2_map_r_iff : forall {A B} {P} {f : A -> B} (l1 l2 : list A),
+    Forall2 P l1 (map f l2) <-> Forall2 (fun x1 x2 => P x1 (f x2)) l1 l2.
+Proof.
+  intros.
+  revert l2.
+  induction l1; intros; split; intro H; inv H.
+  - destruct l2; simpl in *; inv H0.
+    constructor.
+  - constructor.
+  - destruct l2; simpl in *; inv H2.
+    constructor; auto.
+    eapply IHl1; eauto.
+  - constructor; auto.
+    eapply IHl1; eauto.
+Qed.
+
+
+Lemma map_nth_error_inj
+     : forall (A B : Type) (f : A -> B) (n : nat) (l : list A) (d : A),
+       (forall a b, f a = f b -> a = b) ->
+       nth_error l n = Some d <-> nth_error (map f l) n = Some (f d).
+Proof.
+intros.
+revert n.
+induction l; intros.
+- split; intros;
+  apply nth_error_In in H0; inv H0.
+- split; intros;
+    destruct n; simpl in *; inversion H0; auto.
+  apply IHl; auto.
+  f_equal; apply H; auto.
+  apply IHl; auto.
+Qed.
+
+Lemma nth_error_map' :
+  forall (A B : Type) (f : A -> B) (n : nat) (l : list A) (d : B),
+    nth_error (map f l) n = Some d -> exists d', d = f d'.
+Proof.
+  intros; revert n H.
+  induction l; intros.
+  - apply nth_error_In in H.
+    inv H.
+  - destruct n; simpl in *; inversion H.
+    eexists; eauto.
+    eapply IHl; eauto.
+Qed.
+
+Lemma Forall2_nth_error {A B P i vs vs'} {v : A}:
+  nth_error vs i = Some v ->
+  Forall2 P vs vs' ->
+  exists (v' : B),
+    nth_error vs' i = Some v' /\
+    P v v'.
+Proof.
+  intros.
+  revert i v H.
+  induction H0; simpl; intros.
+  - apply nth_error_In in H.
+    inv H.
+  - destruct i; simpl in *; eauto.
+    inv H1.
+    eexists; split; eauto.
+Qed.
+
+Lemma Forall_nth_error {A P i vs} {v : A}:
+  nth_error vs i = Some v ->
+  Forall P vs ->
+    P v.
+Proof.
+  intros.
+  revert i v H.
+  induction H0; simpl; intros.
+  - apply nth_error_In in H.
+    inv H.
+  - destruct i; simpl in *; eauto.
+    inv H1; auto.
+Qed.
+
+Lemma Forall_monotonic {A} (R R' : A -> Prop) (l : list A):
+  (forall x, R x -> R' x) ->
+  Forall R l ->
+  Forall R' l.
+Proof.
+  intros H.
+  induction l as [| x xs IHxs ]; intros Hall.
+  - inv Hall; eauto.
+  - inv Hall. constructor; eauto.
+Qed.
+
+Lemma Disjoint_FromList_cons_l {A} : forall {xs a S},
+  Disjoint A (FromList (a :: xs)) S ->
+  Disjoint A (FromList xs) S.
+Proof.
+  intros.
+  inv H; constructor; intros x Hc.
+  apply (H0 x).
+  unfold Ensembles.In, FromList in *.
+  inv Hc.
+  constructor; auto.
+  unfold Ensembles.In.
+  apply in_cons; auto.
+Qed.
+
+Lemma Disjoint_FromList_cons_r {A} : forall {xs a S},
+  ~ (In a xs) ->
+  Disjoint A (FromList xs) S ->
+  Disjoint A (FromList xs) (a |: S).
+Proof.
+  intros.
+  inv H0; constructor; intros x Hc.
+  inv Hc.
+  inv H2.
+  - inv H3.
+    unfold Ensembles.In, FromList in *.
+    contradiction.
+  - apply (H1 x).
+    constructor; unfold Ensembles.In, FromList in *; auto.
+Qed.
+
+Lemma not_In_cons_Union {A a xs Γ} {x : A}:
+  (x \in (FromList (a :: xs) :|: Γ)) ->
+  a <> x ->
+  (x \in (FromList xs :|: Γ)).
+Proof.
+  intros.
+  inv H.
+  - inv H1; try contradiction.
+    apply Union_introl; auto.
+  - apply Union_intror; auto.
+Qed.
+
+
+Lemma set_lists_In {A} :
+  forall {xs vs x ρ ρ'},
+    In x xs ->
+    @set_lists A xs vs ρ = Some ρ' ->
+    exists v, In v vs /\ M.get x ρ' = Some v.
+Proof.
+  intros xs.
+  induction xs; simpl; intros; try contradiction.
+  destruct vs; try discriminate.
+  destruct (set_lists xs vs ρ) eqn:Heq1; try discriminate.
+  inv H0.
+  inv H; subst.
+  - rewrite M.gss in *; auto.
+    eexists; split; eauto.
+    apply in_eq.
+  - edestruct IHxs as [v [Hin Heqv]]; eauto.
+    destruct (M.elt_eq a x); subst.
+    + rewrite M.gss in *; auto.
+      eexists; split; eauto.
+      apply in_eq.
+    + rewrite M.gso in *; auto.
+      eexists; split; eauto.
+      apply in_cons; auto.
+Qed.
+
+Lemma set_lists_In2 {A} :
+  forall {xs vs x ρ1 ρ2 ρ3 ρ4},
+    In x xs ->
+    @set_lists A xs vs ρ1 = Some ρ2 ->
+    @set_lists A xs vs ρ3 = Some ρ4 ->
+    exists v, In v vs /\ M.get x ρ2 = Some v /\ M.get x ρ4 = Some v.
+Proof.
+  intros xs.
+  induction xs; simpl; intros; try contradiction.
+  destruct vs; try discriminate.
+  destruct (set_lists xs vs ρ1) eqn:Heq1; try discriminate.
+  destruct (set_lists xs vs ρ3) eqn:Heq2; try discriminate.
+  inv H0; inv H1.
+  inv H; subst.
+  - rewrite M.gss in *; auto.
+    rewrite M.gss in *; auto.
+    eexists; repeat (split; eauto).
+    apply in_eq.
+  - edestruct IHxs with (ρ2 := t) (ρ4 := t0) as [v [Hin [Heqv1 Heqv2]]]; eauto.
+    destruct (M.elt_eq a x); subst.
+    + rewrite M.gss in *; auto.
+      rewrite M.gss in *; auto.
+      eexists; repeat (split; eauto).
+      apply in_eq.
+    + rewrite M.gso in *; auto.
+      rewrite M.gso in *; auto.
+      eexists; repeat (split; eauto).
+      apply in_cons; auto.
+Qed.
+
+Lemma set_set {A} {x y} {v : A} {u : A} {ρ} :
+  x <> y ->
+  M.set x v (M.set y u ρ) = M.set y u (M.set x v ρ).
+Proof.
+  intros.
+  apply M.extensionality.
+  intros.
+  destruct (var_dec x i); subst.
+  - rewrite M.gss; auto.
+    destruct (var_dec y i); subst;
+      try contradiction.
+    rewrite M.gso; auto.
+    rewrite M.gss; auto.
+  - rewrite M.gso; auto.
+    destruct (var_dec y i); subst.
+    + repeat rewrite M.gss; auto.
+    + repeat (rewrite M.gso; auto).
+Qed.
+
+(*
+Lemma set_set_eq {A} {x} {v : A} {u : A} {ρ} :
+  M.set x v (M.set x u ρ) = M.set x v ρ.
+Proof.
+  apply M.extensionality.
+  intros.
+  destruct (var_dec x i); subst.
+  - repeat rewrite M.gss; auto.
+  - repeat (rewrite M.gso; auto).
+Qed.
+*)
+
+Lemma set_lists_set {A} :
+  forall {xs vs x v ρ1 ρ2},
+    ~ In x xs ->
+    @set_lists A xs vs ρ1 = Some ρ2 ->
+    set_lists xs vs (M.set x v ρ1) = Some (M.set x v ρ2).
+Proof.
+  intro xs.
+  induction xs; simpl; intros;
+    destruct vs; try discriminate.
+  - inv H0; auto.
+  - destruct (set_lists xs vs ρ1) eqn:Heq1; try discriminate.
+    inv H0.
+    assert (~ In x xs) by (intros Hc; apply H; right; auto).
+    assert (a <> x) by (intros Hc; apply H; left; auto).
+    erewrite IHxs; eauto.
+    f_equal.
+    eapply set_set; eauto.
+Qed.
+
+Lemma FromList_cons_assoc {A} {x : A} l Γ:
+  FromList (x :: l) :|: Γ \subset x |: (FromList l :|: Γ).
+Proof.
+  unfold Ensembles.Included, Ensembles.In, FromList.
+  intros.
+  inv H.
+  + inv H0.
+    apply Union_introl; auto.
+    apply Union_intror; auto.
+  + apply Union_intror.
+    apply Union_intror; auto.
+Qed.
+
+Lemma Forall_fold {A} {P} {l : list A} :
+  fold_right (fun x acc => P x /\ acc) True l <-> Forall P l.
+Proof.
+  induction l; simpl; split; auto; intros.
+  - destruct H; constructor; auto.
+    rewrite <- IHl; auto.
+  - inv H.
+    split; auto.
+    rewrite IHl; auto.
+Qed.
+
+Lemma NoDup_list_norepet:
+  forall {A} (l:list A), NoDup l <-> Coqlib.list_norepet l.
+Proof.
+  intros.
+  induction l; split; intro; auto.
+  constructor. constructor.
+  inv H; constructor; eauto.
+  apply  IHl. auto.
+  inv H; constructor; auto.
+  apply IHl. auto.
+Qed.
+
+Lemma keys_NoDup {A} (m : M.t A) :
+  NoDup (List.map fst (M.elements m)).
+Proof.
+  apply NoDup_list_norepet.
+  apply M.elements_keys_norepet.
+Qed.
+
+Lemma Setminus_Included_Union_l {A} {s1 : Ensemble A} {s2 s3} :
+  Decidable s2 ->
+  s1 \\ s2 \subset s3 ->
+  s1 \subset (s2 :|: s3).
+Proof.
+  intros.
+  unfold Ensembles.Included, Ensembles.In, Ensembles.Setminus in *.
+  intros.
+  inv X.
+  destruct (Dec x).
+  - apply Union_introl; auto.
+  - apply Union_intror.
+    eapply H; eauto.
+Qed.
+
+
+Section All2.
+    Context (A : Type) (B : Type) (R : A -> B -> Prop).
+
+    (* A Fixpoint version of List.Forall2 *)
+    Fixpoint all2 l1 l2 : Prop :=
+      match l1, l2 with
+      | [], [] => True
+      | [] , _::_ => False
+      | _::_, [] => False
+      | a::l1', b::l2' => R a b /\ all2 l1' l2'
+      end.
+
+    Lemma all2_Forall2 l1 l2 : all2 l1 l2 <-> Forall2 R l1 l2.
+    Proof.
+      revert l2.
+      induction l1; simpl in *.
+      - destruct l2; split; intros; auto; try tauto.
+        inv H.
+      - destruct l2; split; intros; auto; try tauto.
+        inv H.
+        destruct H.
+        constructor; auto.
+        apply IHl1; auto.
+        inv H.
+        split; auto.
+        apply IHl1; auto.
+    Qed.
+End All2.
+
+
+Section TreeForall.
+Context {A : Type}
+        {P : A -> Prop}.
+
+Inductive tree_Forall' : (M.tree' A) -> Prop :=
+| Forall_Node001 : forall r, tree_Forall' r -> tree_Forall' (M.Node001 r)
+| Forall_Node010 : forall x, P x -> tree_Forall' (M.Node010 x)
+| Forall_Node011 : forall x r, P x -> tree_Forall' r -> tree_Forall' (M.Node011 x r)
+| Forall_Node100 : forall l, tree_Forall' l -> tree_Forall' (M.Node100 l)
+| Forall_Node101 : forall l r, tree_Forall' l -> tree_Forall' r -> tree_Forall' (M.Node101 l r)
+| Forall_Node110 : forall l x, tree_Forall' l -> P x -> tree_Forall' (M.Node110 l x)
+| Forall_Node111 : forall l x r, tree_Forall' l -> P x -> tree_Forall' r -> tree_Forall' (M.Node111 l x r).
+
+Hint Constructors tree_Forall' : core.
+
+Inductive tree_Forall : (M.tree A) -> Prop :=
+| Forall_Empty : tree_Forall M.Empty
+| Forall_Nodes : forall m', tree_Forall' m' -> tree_Forall (M.Nodes m').
+
+Hint Constructors tree_Forall : core.
+
+Lemma tree_Forall_prop : forall m, tree_Forall m -> (forall x v, m ! x = Some v -> P v).
+Proof.
+  intros m H x v.
+  induction H; intros.
+  - rewrite M.gempty in *.
+    inversion H.
+  - unfold M.get in *.
+    revert x v H0.
+    induction H; intros y v; intros; simpl in *; destruct y; simpl in *; eauto;
+      match goal with
+      | [H : None = Some _ |- _] => inversion H
+      | [H : Some _ = None |- _] => inversion H
+      | [H : Some _ = Some _ |- _] => inversion H; subst; auto
+      end.
+Qed.
+
+End TreeForall.
+
+Lemma map'_ignore : forall {A B} {f : A -> B} {t i j},
+    M.map' (fun _ v => f v) t i = M.map' (fun _ v => f v) t j.
+Proof.
+  induction t; simpl; intros; f_equal; try eapply IHt; try eapply IHt1; try eapply IHt2.
+Qed.
+
+
+Lemma get_list_M_set_Disjoint : forall {A : Type} xs x {v : A} (ρ : M.t A),
+    (~ In x xs) ->
+    get_list xs (M.set x v ρ) = get_list xs ρ.
+Proof.
+  induction xs; intros; simpl in *; auto.
+  rewrite M.gso in *; auto.
+  destruct (ρ ! a); auto.
+  erewrite IHxs; auto.
+Qed.
+
+Lemma M_get_set_eq : forall {A : Type} x (v : A) (ρ : M.t A),
+    ρ ! x = Some v -> M.set x v ρ = ρ.
+Proof.
+  intros.
+  eapply M.extensionality.
+  intro.
+  destruct (var_dec x i); subst.
+  - rewrite M.gss; auto.
+  - rewrite M.gso; auto.
+Qed.
+
+Lemma bool_dec : forall b, b = true \/ b = false.
+Proof.
+  intros; destruct b; auto.
+Qed.
+
+Lemma In_dec : forall {A : Type} {xs : list A} {x : A}, (forall x y : A, {x = y} + {x <> y}) -> (In x xs \/ ~ In x xs).
+Proof.
+  intros A xs x A_dec; revert x.
+  induction xs; intros; simpl in *; try tauto.
+  destruct (A_dec x a); subst.
+  - eapply or_introl; auto.
+  - destruct (IHxs x).
+    + eapply or_introl.
+      eapply or_intror; auto.
+    + eapply or_intror.
+      intro; apply H.
+      destruct H0; subst; try tauto.
+Qed.
+
+Lemma set_lists_length_2:
+  forall {A : Type} {xs1 xs2 : list map_util.M.elt} {rho1 rho1' rho2 : map_util.M.t A} {vs1 vs2 : list A},
+  set_lists xs1 vs1 rho1 = Some rho1' ->
+  length xs1 = length xs2 ->
+  length vs1 = length vs2 ->
+  exists rho2' : map_util.M.t A, set_lists xs2 vs2 rho2 = Some rho2'.
+Proof.
+  induction xs1; intros; destruct xs2; simpl in *; try lia.
+  - destruct vs1; destruct vs2; simpl in *; try lia.
+    eexists; eauto.
+    inv H.
+  - destruct vs1; destruct vs2; simpl in *; try lia.
+    inv H.
+    destruct (set_lists xs1 vs1 rho1) eqn:H2; inv H.
+    edestruct IHxs1 with (xs2 := xs2) (vs1 := vs1) (vs2 := vs2) (rho2 := rho2); eauto.
+    eexists.
+    rewrite H; eauto.
+Qed.
+
+Lemma not_Dom_map_eq {A} (sig:M.t A) x :
+  M.get x sig = None <-> ~ Dom_map sig x.
+Proof.
+  split.
+  - unfold Dom_map.
+    intro. intro Hc.
+    inv Hc.
+    rewrite H0 in H; inv H.
+  - eapply map_util.not_Dom_map_eq; eauto.
+Qed.
+
+Lemma Dom_map_eq {A} (sig:M.t A) x :
+  (exists y, M.get x sig = Some y) <-> Dom_map sig x.
+Proof.
+  unfold Dom_map.
+  split; intros [y Hy]; eauto.
+Qed.
